src/Std/Data/HashSet/IteratorLemmas.lean
@@ -24,7 +24,7 @@ variable {α : Type u} {m : Raw α}
 
 public theorem toList_iter [BEq α] [Hashable α] [EquivBEq α] [LawfulHashable α] (h : m.WF) :
     m.iter.toList = m.toList := by
-  simp [toList, iter, DHashMap.Raw.toList_entriesIter,
+  simp [toList, iter, DHashMap.Raw.toList_iter,
     ← HashMap.Raw.map_fst_toList_eq_keys h.out, HashMap.Raw.toList_inner]
 
 public theorem toListRev_iter [BEq α] [Hashable α] [EquivBEq α] [LawfulHashable α] (h : m.WF) :
@@ -44,14 +44,14 @@ variable {α : Type u} [BEq α] [Hashable α] {m : HashSet α}
 
 public theorem toList_iter [EquivBEq α] [LawfulHashable α] :
     m.iter.toList = m.toList := by
-  simp [iter, DHashMap.toList_entriesIter, toList, HashMap.keys_inner]
+  simp [iter, DHashMap.toList_iter, toList, HashMap.keys_inner]
 
 public theorem toListRev_iter [EquivBEq α] [LawfulHashable α] :
     m.iter.toListRev = m.toList.reverse := by
-  simp [iter, DHashMap.toListRev_entriesIter, toList, HashMap.keys_inner]
+  simp [iter, DHashMap.toListRev_iter, toList, HashMap.keys_inner]
 
 public theorem toArray_iter [EquivBEq α] [LawfulHashable α] :
     m.iter.toArray = m.toArray := by
-  simp [iter, DHashMap.toArray_entriesIter, toArray, HashMap.keysArray]
+  simp [iter, DHashMap.toArray_iter, toArray, HashMap.keysArray]
 
 end Std.HashSet
